MathematicalLogic/FirstOrder/Encoding.lean
@@ -1,0 +1,169 @@
+import MathematicalLogic.FirstOrder.Proof
+
+namespace FirstOrder.Language
+
+variable {𝓛 : Language}
+
+section
+
+variable [∀ n, Encodable (𝓛.Func n)]
+
+def Term.encode : 𝓛.Term n → ℕ
+| #x => 2 * x
+| func (m := m) f v => 2 * m.pair ((Encodable.encode f).pair (Vec.paired λ i => (v i).encode)) + 1
+
+mutual
+def Term.decode (n k : ℕ) : Option (𝓛.Term n) :=
+  if k.bodd then do
+    let m := k.div2.unpair.1
+    match @Encodable.decode (𝓛.Func m) _ k.div2.unpair.2.unpair.1 with
+    | some f => do
+      let v ← decodeVec n k.div2.unpair.2.unpair.2 m
+      some (f ⬝ₜ v)
+    | _ => none
+  else
+    if h : k.div2 < n then
+      some #⟨_, h⟩
+    else none
+termination_by (k, 0)
+decreasing_by
+  simp_wf; simp [Prod.lex_def]
+  apply Nat.lt_of_le_of_lt (Nat.unpair_right_le _)
+  apply Nat.lt_of_le_of_lt (Nat.unpair_right_le _)
+  apply Nat.binaryRec_decreasing
+  intro h; subst h; contradiction
+
+def Term.decodeVec (n k : ℕ) : (m : ℕ) → Option (Vec (𝓛.Term n) m)
+| 0 => if k = 0 then some []ᵥ else none
+| m + 1 => do
+  let t ← decode n k.unpair.1
+  let v ← decodeVec n k.unpair.2 m
+  some (t ∷ᵥ v)
+termination_by m => (k, m)
+decreasing_by
+  all_goals simp_wf; simp [Prod.lex_def]
+  · exact Nat.lt_or_eq_of_le (Nat.unpair_left_le k)
+  · exact Nat.lt_or_eq_of_le (Nat.unpair_right_le k)
+end
+
+theorem Term.encode_decode {t : 𝓛.Term n} : decode n t.encode = some t := by
+  induction t with simp [encode, decode, Nat.div2_val]
+  | @func m f v ih =>
+    rw [Nat.div2_val, Nat.mul_add_div]
+    · simp; rw [Nat.unpair_pair]; simp [Option.bind_eq_some]; clear f
+      induction m with simp [decodeVec, Vec.paired]
+      | zero => simp [Vec.eq_nil]
+      | succ m ih' =>
+        simp [Vec.head, Vec.tail, ih, Function.comp]
+        rw [ih']
+        · simp; nth_rw 3 [Vec.eq_cons v]; rfl
+        · intro; apply ih
+    · simp
+
+instance : Encodable (𝓛.Term n) where
+  encode := Term.encode
+  decode := Term.decode n
+  encodek _ := Term.encode_decode
+
+@[simp] theorem Term.encode_var : Encodable.encode (#x : 𝓛.Term n) = 2 * x := rfl
+@[simp] theorem Term.encode_func {v : Vec (𝓛.Term n) m} :
+  Encodable.encode (f ⬝ₜ v) = 2 * m.pair ((Encodable.encode f).pair (Encodable.encode v)) + 1 := rfl
+
+variable [∀ n, Encodable (𝓛.Rel n)]
+
+def Formula.encode : 𝓛.Formula n → ℕ
+| rel (m := m) r v => 4 * m.pair ((Encodable.encode r).pair (Vec.paired λ i => (v i).encode)) + 1
+| t₁ ≐ t₂ => 4 * Nat.pair t₁.encode t₂.encode + 2
+| ⊥ => 0
+| p ⇒ q => 4 * Nat.pair p.encode q.encode + 3
+| ∀' p => 4 * p.encode + 4
+
+def Formula.decode (n k : ℕ) : Option (𝓛.Formula n) :=
+  match k with
+  | 0 => some ⊥
+  | k + 1 =>
+    match h : k % 4 with
+    | 0 =>
+      let m := (k / 4).unpair.1
+      match @Encodable.decode (𝓛.Rel m) _ (k / 4).unpair.2.unpair.1 with
+      | some r => do
+        let v ← Term.decodeVec n (k / 4).unpair.2.unpair.2 m
+        some (r ⬝ᵣ v)
+      | _ => none
+    | 1 => do
+      let t₁ ← Term.decode n (k / 4).unpair.1
+      let t₂ ← Term.decode n (k / 4).unpair.2
+      some (t₁ ≐ t₂)
+    | 2 => do
+      let p ← decode n (k / 4).unpair.1
+      let q ← decode n (k / 4).unpair.2
+      some (p ⇒ q)
+    | 3 => do
+      let p ← decode (n + 1) (k / 4)
+      some (∀' p)
+    | _ + 4 => none
+termination_by k
+decreasing_by
+  all_goals simp_wf; simp [Nat.lt_succ]
+  · apply le_trans (Nat.unpair_left_le _); apply Nat.div_le_self
+  · apply le_trans (Nat.unpair_right_le _); apply Nat.div_le_self
+  · apply Nat.div_le_self
+
+theorem Formula.encode_decode {p : 𝓛.Formula n} : decode n p.encode = some p := by
+  induction p with simp [encode, decode]
+  | @rel m _ r v =>
+    rw [Nat.mul_mod_right 4]; simp
+    rw [Nat.mul_div_right, Nat.unpair_pair]
+    · simp [Option.bind_eq_some]; clear r
+      induction m with simp [Term.decodeVec, Vec.paired]
+      | zero => simp [Vec.eq_nil]
+      | succ m ih =>
+      simp [Vec.head, Vec.tail, Term.encode_decode, Function.comp, ih]
+      nth_rw 3 [Vec.eq_cons v]; rfl
+    · simp
+  | eq t₁ t₂ =>
+    rw [Nat.mul_add_mod]; simp [Nat.mul_add_div, Term.encode_decode]
+  | imp p q ih₁ ih₂ =>
+    rw [Nat.mul_add_mod]; simp [Nat.mul_add_div, ih₁, ih₂]
+  | all p ih =>
+    rw [Nat.mul_add_mod]; simp [Nat.mul_add_div, ih]
+
+instance : Encodable (𝓛.Formula n) where
+  encode := Formula.encode
+  decode := Formula.decode n
+  encodek _ := Formula.encode_decode
+
+@[simp] theorem Formula.encode_rel {v : Vec (𝓛.Term n) m} :
+  Encodable.encode (r ⬝ᵣ v) = 4 * m.pair ((Encodable.encode r).pair (Encodable.encode v)) + 1 := rfl
+@[simp] theorem Formula.encode_eq {t₁ t₂ : 𝓛.Term n} :
+  Encodable.encode (t₁ ≐ t₂) = 4 * (Encodable.encode t₁).pair (Encodable.encode t₂) + 2 := rfl
+@[simp] theorem Formula.encode_false :
+  Encodable.encode (⊥ : 𝓛.Formula n) = 0 := rfl
+@[simp] theorem Formula.encode_imp {p q : 𝓛.Formula n} :
+  Encodable.encode (p ⇒ q) = 4 * (Encodable.encode p).pair (Encodable.encode q) + 3 := rfl
+@[simp] theorem Formula.encode_all {p : 𝓛.Formula (n + 1)} :
+  Encodable.encode (∀' p) = 4 * Encodable.encode p + 4 := rfl
+
+lemma Formula.encode_lt_imp_left {p q : 𝓛.Formula n} : Encodable.encode p < Encodable.encode (p ⇒ q) := by
+  simp [Nat.lt_succ]
+  apply le_trans' (Nat.le_add_right _ _)
+  apply le_trans' (Nat.le_mul_of_pos_left _ (by simp))
+  apply Nat.left_le_pair
+
+lemma Formula.encode_lt_imp_right {p q : 𝓛.Formula n} : Encodable.encode q < Encodable.encode (p ⇒ q) := by
+  simp [encode, Nat.lt_succ]
+  apply le_trans' (Nat.le_add_right _ _)
+  apply le_trans' (Nat.le_mul_of_pos_left _ (by simp))
+  apply Nat.right_le_pair
+
+end
+
+section
+variable [∀ n, Countable (𝓛.Func n)] [∀ n, Countable (𝓛.Rel n)]
+noncomputable scoped instance : Encodable (𝓛.Func n) := Encodable.ofCountable _
+noncomputable scoped instance : Encodable (𝓛.Rel n) := Encodable.ofCountable _
+instance : Countable (𝓛.Term n) := inferInstance
+instance : Countable (𝓛.Formula n) := inferInstance
+end
+
+end FirstOrder.Language
